common/FlatComp.v
@@ -11,80 +11,47 @@ Open Scope smallstep_scope.
 Delimit Scope smallstep_scope with smallstep.
 
 Section FLAT_COMP.
-  Context {liA liB} (L1: semantics liA liB) (L2: semantics liA liB).
+  Context {I liA liB} (L: I -> semantics liA liB).
   Section WITH_SE.
-    Context (se: Genv.symtbl) (qset: ident -> Prop).
+    Context (se: Genv.symtbl).
 
-    Variant flat_state :=
-    | flat_st1 (s: state L1)
-    | flat_st2 (s: state L2).
+    Variant flat_state := flat_st i (s: state (L i)).
 
     Inductive flat_step: flat_state -> trace -> flat_state -> Prop :=
-    | step1 s t s':
-        Step (L1 se) s t s' -> flat_step (flat_st1 s) t (flat_st1 s')
-    | step2 s t s':
-        Step (L2 se) s t s' -> flat_step (flat_st2 s) t (flat_st2 s').
+    | step_internal i s t s':
+        Step (L i se) s t s' -> flat_step (flat_st i s) t (flat_st i s').
 
     Inductive flat_initial_state (q: query liB): flat_state -> Prop :=
-    | initial_state1 s:
-        initial_state (L1 se) q s ->
-        flat_initial_state q (flat_st1 s)
-    | initial_state2 s:
-        initial_state (L2 se) q s ->
-        flat_initial_state q (flat_st2 s).
+    | initial_state_intro i s:
+        initial_state (L i se) q s ->
+        flat_initial_state q (flat_st i s).
 
     Inductive flat_at_external: flat_state -> query liA -> Prop :=
-    | at_external1 s q:
-        at_external (L1 se) s q ->
-        flat_at_external (flat_st1 s) q
-    | at_external2 s q:
-        at_external (L2 se) s q ->
-        flat_at_external (flat_st2 s) q.
+    | at_external_intro i s q:
+        at_external (L i se) s q -> flat_at_external (flat_st i s) q.
 
     Inductive flat_after_external: flat_state -> reply liA -> flat_state -> Prop :=
-    | after_external1 s r s':
-        after_external (L1 se) s r s' ->
-        flat_after_external (flat_st1 s) r (flat_st1 s')
-    | after_external2 s r s':
-        after_external (L2 se) s r s' ->
-        flat_after_external (flat_st2 s) r (flat_st2 s').
+    | after_external_intro i s r s':
+        after_external (L i se) s r s' ->
+        flat_after_external (flat_st i s) r (flat_st i s').
 
     Inductive flat_final_state: flat_state -> reply liB -> Prop :=
-    | final_state1 s r:
-        final_state (L1 se) s r ->
-        flat_final_state (flat_st1 s) r
-    | final_state2 s r:
-        final_state (L2 se) s r ->
-        flat_final_state (flat_st2 s) r.
+    | final_state1 i s r:
+        final_state (L i se) s r -> flat_final_state (flat_st i s) r.
 
-    Lemma star_internal1 s t s':
-      Star (L1 se) s t s' ->
-      star (fun _ => flat_step) tt (flat_st1 s) t (flat_st1 s').
+    Lemma star_internal i s t s':
+      Star (L i se) s t s' ->
+      star (fun _ => flat_step) tt (flat_st i s) t (flat_st i s').
     Proof.
       induction 1; [eapply star_refl | eapply star_step]; eauto.
       constructor; auto.
     Qed.
 
-    Lemma plus_internal1 s t s':
-      Plus (L1 se) s t s' ->
-      plus (fun _ => flat_step) tt (flat_st1 s) t (flat_st1 s').
+    Lemma plus_internal i s t s':
+      Plus (L i se) s t s' ->
+      plus (fun _ => flat_step) tt (flat_st i s) t (flat_st i s').
     Proof.
-      destruct 1; econstructor; eauto using step1, star_internal1.
-    Qed.
-
-    Lemma star_internal2 s t s':
-      Star (L2 se) s t s' ->
-      star (fun _ => flat_step) tt (flat_st2 s) t (flat_st2 s').
-    Proof.
-      induction 1; [eapply star_refl | eapply star_step]; eauto.
-      constructor; auto.
-    Qed.
-
-    Lemma plus_internal2 s t s':
-      Plus (L2 se) s t s' ->
-      plus (fun _ => flat_step) tt (flat_st2 s) t (flat_st2 s').
-    Proof.
-      destruct 1; econstructor; eauto using step2, star_internal2.
+      destruct 1; econstructor; eauto using step_internal, star_internal.
     Qed.
 
   End WITH_SE.
@@ -101,273 +68,237 @@ Section FLAT_COMP.
           globalenv := tt;
         |};
       skel := sk;
-      footprint i := footprint L1 i \/ footprint L2 i;
+      footprint x := exists i, footprint (L i) x;
     |}.
+
+  (* The external call from (L i) cannot be in the footprint of (L j) for i ≠ j *)
+  Class FlatLinkable :=
+    flat_linking:
+      forall i j se s q, at_external (L i se) s q -> valid_query (L j) se q -> i = j.
 
 End FLAT_COMP.
 
-Definition flat_comp_semantics {liA liB} (L1: semantics liA liB)
-           (L2: semantics liA liB): option (semantics liA liB) :=
-  option_map (flat_comp_semantics' L1 L2) (link (skel L1) (skel L2)).
-
-Notation "L1 ⊎ L2" :=  (flat_comp_semantics L1 L2)(at level 40, left associativity): lts_scope.
-
 Section FSIM.
-  Context {liA1 liA2 liB1 liB2}
-          (cc1: callconv liA1 liB1)
-          (cc2: callconv liA2 liB2)
-          (L1 L2: semantics liA1 liA2)
-          (L1' L2': semantics liB1 liB2).
-  Context (HL1: fsim_components cc1 cc2 L1 L1')
-          (HL2: fsim_components cc1 cc2 L2 L2')
+  Context {I liA1 liA2 liB1 liB2}
+          (cc1: callconv liA1 liA2)
+          (cc2: callconv liB1 liB2)
+          (L1: I -> semantics liA1 liB1)
+          (L2: I -> semantics liA2 liB2).
+  Context (HL: forall i, fsim_components cc1 cc2 (L1 i) (L2 i))
           (se1 se2: Genv.symtbl) (w : ccworld cc2)
           (Hse: match_senv cc2 w se1 se2)
-          (Hse1: Genv.valid_for (skel L1) se1)
-          (Hse2: Genv.valid_for (skel L2) se1).
+          (Hse1: forall i, Genv.valid_for (skel (L1 i)) se1).
 
-  Variant index := | index1 (i: fsim_index HL1) | index2 (i: fsim_index HL2).
+  Notation index := {i & fsim_index (HL i)}.
   Variant order: index -> index -> Prop :=
-  | order1 i1 i1': fsim_order HL1 i1 i1' -> order (index1 i1) (index1 i1')
-  | order2 i2 i2': fsim_order HL2 i2 i2' -> order (index2 i2) (index2 i2').
+  | order_intro i x y: fsim_order (HL i) x y -> order (existT _ i x) (existT _ i y).
 
-  Variant match_states: index -> flat_state L1 L2 -> flat_state L1' L2' -> Prop :=
-  | match_st1 i s1 s1':
-      fsim_match_states HL1 se1 se2 w i s1 s1' ->
-      match_states (index1 i) (flat_st1 L1 L2 s1) (flat_st1 L1' L2' s1')
-  | match_st2 i s2 s2':
-      fsim_match_states HL2 se1 se2 w i s2 s2' ->
-      match_states (index2 i) (flat_st2 L1 L2 s2) (flat_st2 L1' L2' s2').
+  Variant match_states: index -> flat_state L1 -> flat_state L2 -> Prop :=
+  | match_flat_st i idx s1 s2:
+      fsim_match_states (HL i) se1 se2 w idx s1 s2 ->
+      match_states (existT _ i idx) (flat_st L1 i s1) (flat_st L2 i s2).
 
   Local Lemma flat_compose_simulation' sk sk':
     fsim_properties cc1 cc2 se1 se2 w
-                    (flat_comp_semantics' L1 L2 sk se1)
-                    (flat_comp_semantics' L1' L2' sk' se2)
+                    (flat_comp_semantics' L1 sk se1)
+                    (flat_comp_semantics' L2 sk' se2)
                     index order match_states.
   Proof.
     split; cbn.
     - intros q1 q2 s1 Hq H.
-      inv H;
-        [ pose proof (fsim_lts HL1 _ _ Hse Hse1)
-        | pose proof (fsim_lts HL2 _ _ Hse Hse2)
-        ];
-        edestruct @fsim_match_initial_states as (idx & s' & Hs' & Hs);
+      inv H; pose proof (fsim_lts (HL i) _ _ Hse (Hse1 i)).
+      edestruct @fsim_match_initial_states as (idx & s' & Hs' & Hs);
         eauto; eexists _, _; split; econstructor; eauto.
-    - intros i s1 s2 r1 Hs H.
-      inv H; inv Hs;
-        [ pose proof (fsim_lts HL1 _ _ Hse Hse1)
-        | pose proof (fsim_lts HL2 _ _ Hse Hse2)
-        ];
-        edestruct @fsim_match_final_states as (r' & H' & Hr');
+    - intros idx s1 s2 r1 Hs H.
+      inv H. inv Hs. subst_dep.
+      pose proof (fsim_lts (HL i) _ _ Hse (Hse1 i)).
+      edestruct @fsim_match_final_states as (r' & H' & Hr');
         eauto; eexists; split; try econstructor; eauto.
-    - intros i s1 s2 q1 Hs H.
-      inv H; inv Hs;
-        [ pose proof (fsim_lts HL1 _ _ Hse Hse1)
-        | pose proof (fsim_lts HL2 _ _ Hse Hse2)
-        ];
-        edestruct @fsim_match_external as (w1 & q' & H' & Hq' & Hse' & HH);
+    - intros idx s1 s2 q1 Hs H.
+      inv H. inv Hs. subst_dep.
+      pose proof (fsim_lts (HL i) _ _ Hse (Hse1 i)).
+      edestruct @fsim_match_external as (w1 & q' & H' & Hq' & Hse' & HH);
         eauto; eexists _, _; repeat apply conj; eauto.
       + constructor; auto.
-      + intros r1 r2 fs Hr Haft. inv Haft.
+      + intros r1 r2 fs Hr Haft. inv Haft. subst_dep.
         exploit HH; eauto. intros (? & ? & ? & ?).
         eexists _, _; split; econstructor; eauto.
-      + constructor; auto.
-      + intros r1 r2 fs Hr Haft. inv Haft.
-        exploit HH; eauto. intros (? & ? & ? & ?).
-        eexists _, _; split; econstructor; eauto.
-    - intros s1 t s1' Hstep i s2 Hs.
-      inv Hstep; inv Hs;
-        [ pose proof (fsim_lts HL1 _ _ Hse Hse1)
-        | pose proof (fsim_lts HL2 _ _ Hse Hse2)
-        ];
-        edestruct @fsim_simulation as (idx' & ? & Hs2' & Hs');
-        eauto.
+    - intros s1 t s1' Hstep idx s2 Hs.
+      inv Hstep. inv Hs. subst_dep.
+      pose proof (fsim_lts (HL i) _ _ Hse (Hse1 i)).
+      edestruct @fsim_simulation as (idx' & ? & Hs2' & Hs'); eauto.
       + eexists _, _; split.
         * destruct Hs2'; [left | right].
-          -- apply plus_internal1. eauto.
+          -- apply plus_internal. eauto.
           -- destruct a; split; [ | constructor ]; eauto.
-             apply star_internal1. eauto.
-        * now constructor.
-      + eexists _, _; split.
-        * destruct Hs2'; [left | right].
-          -- apply plus_internal2. eauto.
-          -- destruct a; split; [ | constructor ]; eauto.
-             apply star_internal2. eauto.
+             apply star_internal. eauto.
         * now constructor.
   Qed.
 
 End FSIM.
 
+Require Import ClassicalEpsilon.
+
+Section FLAT_FSIM.
+
+  Context {I liA1 liA2 liB1 liB2}
+          (cc1: callconv liA1 liA2)
+          (cc2: callconv liB1 liB2)
+          (L1: I -> semantics liA1 liB1)
+          (L2: I -> semantics liA2 liB2).
+  Hypothesis (H: forall i, forward_simulation cc1 cc2 (L1 i) (L2 i)).
+  Variable (sk: AST.program unit unit).
+  Hypothesis (Hsk: forall i, linkorder (skel (L1 i)) sk).
+
+  Lemma flat_composition_simulation':
+    forward_simulation cc1 cc2 (flat_comp_semantics' L1 sk) (flat_comp_semantics' L2 sk).
+  Proof.
+    assert (HL: forall i, fsim_components cc1 cc2 (L1 i) (L2 i)).
+    {
+      intros i. specialize (H i).
+      apply epsilon. auto. exact (fun _ => True).
+    }
+    constructor.
+    eapply Forward_simulation
+      with (order cc1 cc2 L1 L2 HL)
+           (match_states cc1 cc2 L1 L2 HL); auto.
+    - cbn. intros id.
+      split; intros [i Hi]; exists i; rewrite (fsim_footprint (HL i)) in *; auto.
+    - intros se1 se2 w Hse Hse1.
+      eapply flat_compose_simulation'; eauto.
+      intros; eapply Genv.valid_for_linkorder; eauto.
+    - clear - HL. intros [i x].
+      induction (fsim_order_wf (HL i) x) as [x Hx IHx].
+      constructor. intros z Hxz. inv Hxz; subst_dep. eauto.
+  Qed.
+
+End FLAT_FSIM.
+
+Definition flat_comp_semantics {liA liB} (L1: semantics liA liB)
+           (L2: semantics liA liB): option (semantics liA liB) :=
+  let L i := match i with true => L1 | false => L2 end in
+  option_map (flat_comp_semantics' L) (link (skel L1) (skel L2)).
+
+Notation "L1 ⊎ L2" :=  (flat_comp_semantics L1 L2)(at level 40, left associativity): lts_scope.
+
 Lemma flat_compose_simulation
       {liA1 liA2 liB1 liB2}
       (cc1: callconv liA1 liB1) (cc2: callconv liA2 liB2)
-      L1 L2 L1' L2' L L':
-  forward_simulation cc1 cc2 L1 L1' ->
-  forward_simulation cc1 cc2 L2 L2' ->
-  L1 ⊎ L2 = Some L -> L1' ⊎ L2' = Some L' ->
-  forward_simulation cc1 cc2 L L'.
+      L1a L2a L1b L2b L1 L2:
+  forward_simulation cc1 cc2 L1a L2a ->
+  forward_simulation cc1 cc2 L1b L2b ->
+  L1a ⊎ L1b = Some L1 -> L2a ⊎ L2b = Some L2 ->
+  forward_simulation cc1 cc2 L1 L2.
 Proof.
   unfold flat_comp_semantics. unfold option_map.  intros [HL1] [HL2] H1 H2.
-  destruct (link (skel L1) (skel L2)) as [sk1|] eqn:Hsk1; try discriminate.
-  inv H1.
-  destruct (link (skel L1') (skel L2')) as [sk2|] eqn:Hsk2; try discriminate.
-  inv H2.
-  constructor.
-  eapply Forward_simulation
-    with (order cc1 cc2 L1 L2 L1' L2' HL1 HL2)
-         (match_states cc1 cc2 L1 L2 L1' L2' HL1 HL2).
-  - cbn. destruct HL1, HL2. congruence.
-  - cbn. intros i. destruct HL1, HL2.
-    rewrite fsim_footprint, fsim_footprint0. reflexivity.
-  - intros se1 se2 w Hse Hse1.
-    pose proof (link_linkorder _ _ _ Hsk1) as [Hsk1a Hsk1b].
-    eapply flat_compose_simulation'; eauto.
-    eapply Genv.valid_for_linkorder; eauto.
-    eapply Genv.valid_for_linkorder; eauto.
-  - clear - HL1 HL2. intros [|].
-    + induction (fsim_order_wf HL1 i). constructor.
-      intros. inv H1. apply H0. auto.
-    + induction (fsim_order_wf HL2 i). constructor.
-      intros. inv H1. apply H0. auto.
+  destruct (link (skel L1a) (skel L1b)) as [sk1|] eqn:Hsk1;
+    try discriminate. inv H1.
+  destruct (link (skel L2a) (skel L2b)) as [sk2|] eqn:Hsk2;
+    try discriminate. inv H2.
+  replace sk2 with sk1.
+  apply flat_composition_simulation'.
+  - intros [|]; constructor; auto.
+  - intros [|]; pose proof (link_linkorder _ _ _ Hsk1) as [? ?]; auto.
+  - destruct HL1, HL2. congruence.
 Qed.
 
 Section APPROX.
 
-  Context {li} (L1 L2: semantics li li).
+  Context {I li} (L: I -> semantics li li).
   Context (sk: AST.program unit unit).
+  Context {HP: forall i, ProgramSem (L i)}.
+  Context `{!FlatLinkable L}.
 
-  Let L := fun i => match i with true => L1 | false => L2 end.
+  Hypothesis I_dec: forall (i j : I), {i = j} + {i <> j}.
 
-  Inductive match_frame: flat_state L1 L2 -> list (SmallstepLinking_.frame L) -> Prop :=
-  | match_frame1 s:
-      match_frame (flat_st1 L1 L2 s) (st L true s :: nil)
-  | match_frame2 s:
-      match_frame (flat_st2 L1 L2 s) (st L false s :: nil).
-
-  Hypothesis flat_linking1:
-    forall se s q, at_external (L2 se) s q -> ~ valid_query L1 se q.
-  Hypothesis flat_linking2:
-    forall se s q, at_external (L1 se) s q -> ~ valid_query L2 se q.
-  Hypothesis extcall_invalid:
-    forall i se s q, Smallstep_.at_external (L i se) s q -> ~ valid_query (L i) se q.
-  Hypothesis valid_initial_state:
-    forall i se q s, initial_state (L i se) q s -> valid_query (L i) se q.
-  (* Hypothesis flat_linking: *)
-  (*   forall i j se q, valid_query (li := li) (L i) se q -> valid_query (L j) se q -> i = j. *)
+  Inductive match_frame: flat_state L -> list (SmallstepLinking_.frame L) -> Prop :=
+  | match_frame_intro i s:
+      match_frame (flat_st L i s) (st L i s :: nil).
 
   Lemma flat_composition_approximation:
-    flat_comp_semantics' L1 L2 sk ≤ SmallstepLinking_.semantics L sk.
+    flat_comp_semantics' L sk ≤ SmallstepLinking_.semantics' L sk.
   Proof.
-    constructor. econstructor; eauto.
-    {
-      intros. split.
-      - intros [|]; [exists true | exists false]; eauto.
-      - intros [[|] ?]; [left | right]; eauto.
-    }
+    constructor. econstructor; eauto. intros. reflexivity.
     intros se ? [ ] [ ] Hse.
     instantiate (1 := fun _ _ _ => _). cbn beta.
     apply forward_simulation_step with (match_states := match_frame).
     - intros q ? s1 [ ] Hs.
       inv Hs; eexists; split; econstructor; eauto.
+      eapply incoming_query_valid; eauto.
     - intros s1 s2 r Hs H.
-      inv H; inv Hs; eexists; split; econstructor; eauto.
+      inv H. inv Hs. subst_dep.
+      eexists; split; econstructor; eauto.
     - intros s1 s2 q1 Hs H.
-      inv H; inv Hs; eexists tt, _; repeat apply conj; try constructor; auto.
-      + intros [|].
-        eapply extcall_invalid. eauto.
-        eapply flat_linking2. eauto.
-      + intros r1 ? s1' [ ] H. inv H.
-        eexists; split; constructor; auto.
-      + intros [|].
-        eapply flat_linking1. eauto.
-        eapply extcall_invalid. eauto.
-      + intros r1 ? s1' [ ] H. inv H.
+      inv H. inv Hs. subst_dep.
+      eexists tt, _; repeat apply conj; try constructor; auto.
+      + intros j. destruct (I_dec i j) eqn: HI.
+        * subst. eapply outgoing_query_invalid. eauto.
+        * intros X. apply n. eapply flat_linking; eauto.
+      + intros r1 ? s1' [ ] H. inv H. subst_dep.
         eexists; split; constructor; auto.
     - intros s1 t s1' Hstep s2 Hs.
-      inv Hstep; inv Hs;
-        eexists; (split; [ | econstructor]; constructor; auto).
+      inv Hstep. inv Hs. subst_dep.
+      eexists; (split; [ | econstructor]; constructor; auto).
     - apply well_founded_ltof.
   Qed.
 
 End APPROX.
 
 Section DIST.
-  Context {liA liB liC} (L1: semantics liB liC) (L2: semantics liB liC)
-          (L: semantics liA liB).
+  Context {I liA liB liC} (Li: I -> semantics liB liC) (L: semantics liA liB).
   Context (sk: AST.program unit unit).
-  Let Lh := flat_comp_semantics' L1 L2 sk.
-  Let Lv1 := comp_semantics' L1 L sk.
-  Let Lv2 := comp_semantics' L2 L sk.
+  Let Lh := flat_comp_semantics' Li sk.
+  Let Lv i := comp_semantics' (Li i) L sk.
+  Hypothesis non_empty: inhabited I.
 
-  Inductive dist_match_state:
-    (comp_state Lh L) -> (flat_state Lv1 Lv2) -> Prop :=
-  | dist_match_state1 s1:
-      dist_match_state (st1 Lh _ (flat_st1 _ L2 s1))
-                       (flat_st1 Lv1 _ (st1 _ L s1))
-  | dist_match_state2 s2:
-      dist_match_state (st1 Lh _ (flat_st2 L1 _ s2))
-                       (flat_st2 _ Lv2 (st1 L2 _ s2))
-  | dist_match_state3 s1 s:
-      dist_match_state (st2 Lh L (flat_st1 L1 L2 s1) s)
-                       (flat_st1 Lv1 Lv2 (st2 L1 L s1 s))
-  | dist_match_state4 s2 s:
-      dist_match_state (st2 Lh L (flat_st2 L1 L2 s2) s)
-                       (flat_st2 Lv1 Lv2 (st2 L2 L s2 s)).
+  (* (L1 ⊎ L2 ⊎ ... ) ∘ L ≅ (L1 ∘ L) ⊎ (L2 ∘ L) ⊎ ... *)
+  Inductive dist_match_state: comp_state Lh L -> flat_state Lv -> Prop :=
+  | dist_match_state1 i s:
+      dist_match_state (st1 Lh _ (flat_st Li i s))
+                       (flat_st Lv i (st1 _ L s))
+  | dist_match_state2 i s1 s2:
+      dist_match_state (st2 Lh L (flat_st Li i s1) s2)
+                       (flat_st Lv i (st2 (Li i) L s1 s2)).
+
+  Hint Constructors dist_match_state
+       flat_initial_state flat_at_external
+       flat_final_state flat_after_external
+       comp_initial_state comp_at_external
+       comp_after_external comp_final_state.
 
   Ltac esca := eexists; split; repeat constructor; auto.
-
   (* (L1 ⊎ L2) ∘ L ≤ (L1 ∘ L) ⊎ (L2 ∘ L) *)
   Lemma distributivity1:
-    comp_semantics' Lh L sk ≤ flat_comp_semantics' Lv1 Lv2 sk.
+    comp_semantics' Lh L sk ≤ flat_comp_semantics' Lv sk.
   Proof.
-    constructor. econstructor; eauto. intros i. firstorder.
+    constructor. econstructor; eauto. intros id. firstorder.
     intros se ? [ ] [ ] Hse.
     instantiate (1 := fun _ _ _ => _). cbn beta.
     eapply forward_simulation_step with (match_states := dist_match_state).
     - intros q1 ? s1 [ ] H.
-      inv H; inv H0; eexists; split; constructor; auto.
-      (* + destruct H as [? [? [? ?]]]. split; auto. *)
-      (*   eexists; split; eauto. apply or_introl; auto. *)
-      + now constructor.
-      (* + destruct H as [? [? [? ?]]]. split; auto. *)
-      (*   eexists; split; eauto. apply or_introl; auto. *)
-      + now constructor.
-    - intros s1 s2 r1 Hs H.
-      inv H; inv H0; inv Hs; esca.
+      inv H. inv H0. eexists; split; auto.
+      repeat constructor. auto.
+    - intros s1 s2 r1 Hs H. inv H; inv H0; inv Hs. subst_dep. esca.
     - intros s1 s2 q1 Hs H.
-      inv H; inv Hs; eexists tt, _; repeat apply conj; try constructor; auto.
-      + constructor; auto.
-      + intros r1 ? s1' [ ] H. inv H. esca.
+      inv H. inv Hs.
+      eexists tt, _; repeat apply conj; try constructor; auto.
       + constructor; auto.
       + intros r1 ? s1' [ ] H. inv H. esca.
     - intros s1 t s1' Hstep s2 Hs.
       inv Hstep; inv Hs.
-      + inv H. esca.
-      + inv H. esca.
+      + inv H. subst_dep. esca.
       + esca.
-      + esca.
-      + inv H. eexists; split. constructor. eapply step_push; eauto.
-        constructor.
-      + inv H. eexists; split. constructor. eapply step_push; eauto.
-        constructor.
-      + inv H0. eexists; split. constructor. eapply step_pop; eauto.
-        constructor.
-      + inv H0. eexists; split. constructor. eapply step_pop; eauto.
-        constructor.
+      + inv H. subst_dep.
+        eexists; split; auto. constructor. eapply step_push; eauto.
+      + inv H0. subst_dep.
+        eexists; split; auto. constructor. eapply step_pop; eauto.
     - apply well_founded_ltof.
   Qed.
-
-  (* (* This is required because L1 ∘ L2 doesn't use valid_query to ensure the *) *)
-  (* (*    query invokes execution is within the footprint. Otherwise, the identity *) *)
-  (* (*    transition would be meaningless *) *)
-  (* Hypothesis init_state_valid1: *)
-  (*   forall se q s, initial_state (L1 se) q s -> valid_query L1 se q. *)
-  (* Hypothesis init_state_valid2: *)
-  (*   forall se q s, initial_state (L2 se) q s -> valid_query L2 se q. *)
 
   Ltac esca' := eexists; split; [ | constructor]; repeat constructor; auto.
   (* (L1 ∘ L) ⊎ (L2 ∘ L) ≤ (L1 ⊎ L2) ∘ L *)
   Lemma distributivity2:
-    flat_comp_semantics' Lv1 Lv2 sk ≤ comp_semantics' Lh L sk.
+    flat_comp_semantics' Lv sk ≤ comp_semantics' Lh L sk.
   Proof.
     constructor. econstructor; eauto. intros i. firstorder.
     intros se ? [ ] [ ] Hse.
@@ -375,31 +306,23 @@ Section DIST.
     eapply forward_simulation_step with
         (match_states := fun s1 s2 => dist_match_state s2 s1).
     - intros q1 ? s1 [ ] H. inv H; inv H0; esca'.
-    - intros s1 s2 r1 Hs H. inv H; inv H0; inv Hs; esca'.
+    - intros s1 s2 r1 Hs H. inv H; inv H0; inv Hs; subst_dep; esca'.
     - intros s1 s2 q1 Hs H.
       inv H; inv H0; inv Hs; eexists tt, _; repeat apply conj;
-        try constructor; auto.
-      + intros r1 ? s1' [ ] Hx. inv Hx. inv H1; esca'.
-      + intros r1 ? s1' [ ] Hx. inv Hx. inv H1; esca'.
+        try constructor; auto. subst_dep.
+      intros r1 ? s1' [ ] Hx. inv Hx.
+      subst_dep. inv H4. esca'.
     - intros s1 t s1' Hstep s2 Hs.
-      inv Hstep; inv H; inv Hs.
+      inv Hstep; inv H; inv Hs; subst_dep.
       + esca'.
       + esca'.
-      + eexists. split; [ | constructor ].
-        eapply step_push; eauto; try constructor; auto; firstorder.
-      + eexists. split; [ | constructor ].
-        eapply step_pop; eauto; try constructor; auto; firstorder.
-      + esca'.
-      + esca'.
-      + esca'.
-        eapply step_push; eauto; try constructor; auto; firstorder.
-      + esca'.
-        eapply step_pop; eauto; try constructor; auto; firstorder.
+      + esca'. eapply step_push; eauto. now constructor.
+      + esca'. eapply step_pop; eauto. now constructor.
     - apply well_founded_ltof.
   Qed.
 
   Theorem flat_categorical_comp_distributivity:
-    flat_comp_semantics' Lv1 Lv2 sk ≡ comp_semantics' Lh L sk.
+    flat_comp_semantics' Lv sk ≡ comp_semantics' Lh L sk.
   Proof.
     split; [ exact distributivity2 | exact distributivity1 ].
   Qed.
